% To submit: 3, 6, 9
% Author: Jonah Laurence

We are to solve the following differential equations by separation of variables.
\begin{enumerate}
	\item[\textbf{3.}]
		We are given this differential equation.
		\[(y-3)\dydx = \frac{4y}{x}\]
		After rearranging and integrating we obtain the following.
		\begin{gather*}
			\frac{(y-3)\dydx}{y} = \frac{4}{x}\\
			\dydx - \frac{3\dydx}{y} = \frac{4}{x}\\
			\int \dydx - \frac{3\dydx}{y} dx = \int \frac{4}{x} dx\\
		\end{gather*}

		From integration by substitution,
		\begin{gather*}
			\int 1 - \frac{3}{y} dy = \int \frac{4}{x} dx\\
			y - 3 \ln y = 4 \ln x + c\\
			\frac{y}{4} - \ln y^{\frac{3}{4}} = \ln x + c\\
			\ln x + \ln y^{\frac{3}{4}} = \frac{y}{4} - c\\
			\ln xy^{\frac{3}{4}} = \frac{y}{4} - c\\
			xy^{\frac{3}{4}}  = e^{\frac{y}{4} - c}
		\end{gather*}
		Let \(\tilde{c} \equiv \frac{1}{e^c}\).
		\[xy^{\frac{3}{4}} = \tilde{c} e^{\frac{y}{4}}\]

	\item[\textbf{6.}]
		We are given this differential equation.
		\[\cos^2 (x) y'(x) = y + 3\]

		Now we rearrange and integrate to obtain the following.
		\begin{gather*}
			\frac{y'(x)}{y+3} = \frac{1}{\cos^2 x}\\
			\int \frac{y'(x)}{y+3} dx = \int \frac{1}{\cos^2 x} dx\\
			\int \frac{1}{y+3} dy = \tan x + c\\
			\ln \vert y+3 \vert = \tan x + c\\
			y + 3 = e^{\tan x + c}
		\end{gather*}

		Let \(\tilde{c} \equiv e^c\). Finally we have
		\[y = \tilde{c} e^{\tan x} - 3\]

	\item[\textbf{9.}]
		We are given this differential equation.
		\[y'(x) = 3x^2 (y+2)\]

		After rearranging and integrating we obtain the following.
		\begin{gather}
			y' = 3x^2 (y+2)\\
			\frac{y'}{y+2} = 3x^2\\
			\int \frac{y'}{y+2}\ dx = \int 3x^2\ dx\\
			\int \frac{1}{y+2}\ dy = x^3 + c\\
			\ln \vert y+2 \vert = x^3 + c\\
			y + 2 = e^{x^3 + c}
		\end{gather}

		Let \(\tilde{c} \equiv e^c\). Now we have
		\[y = \tilde{c} e^{x^3} - 2\]

\end{enumerate}