% To submit: 1, 4
% Author: Jonah Laurence

We are to solve the following differential equations, finding a general solution and a particular solution with the given initial condition. (Note that the right-hand side depends on \(x\) only.)
\begin{enumerate}
	\item[\textbf{1.}]
		We are given this equation and initial condition.
		\[\dydx = 3x^2 + 5, \qquad y(1) = 1\]

		Now we can integrate \(\dydx\) to obtain \(y\).
		\[
			\int \dydx dx = \int (3x^2 + 5) dx
		\]

		The general solution is
		\[
			y(x) = x^3 + 5x + c
		\]

		Now we can substitute our initial condition
		\[
			y(1) = 1^3 + 5(1) + c = 1\ \Rightarrow\ c = -5
		\]

		The particular solution is
		\[
			y(x) = x^3 + 5x - 5 \\
		\]

	\item[\textbf{4.}]
		We are given this equation and initial condition.
		\[\dydx = \ln \left| x-1 \right|, \hspace{1em} y(0) = 1\]
		Now we can integrate \(\dydx\) to obtain \(y\).
		\[
			\int \dydx dx = \int (\ln \left| x-1 \right|) dx
		\]
		The general solution is
		\[
			y(x) = (x-1) \ln \left| x-1 \right| - x + c
		\]

		Now we can substitute our initial condition
		\[
			y(0) = (-1) \ln \left| -1 \right| + c = 1\ \Rightarrow\ c = 1
		\]

		The particular solution is
		\[
			y(x) = (x-1) \ln \left| x-1 \right| - x + 1
		\]

\end{enumerate}