% To submit: 3, 5, 7, 9
% Author: Jonah Laurence

We must solve the following differential equations, using the method of integration-factor.
\begin{enumerate}
	\item[\textbf{3.}]
		\(y'(x) + \left[\frac{1}{x}+1\right]y = e^x\).
		\begin{gather*}
			y'(x) + \left[\frac{1}{x}+1\right]y = e^x\\
			\alpha (x) = \exp\left[\int \frac{1}{x}+1dx\right]
			= \exp\left[\ln x + x\right] = x e^x
		\end{gather*}

		Multiply both sides by the integrating factor, \(\alpha (x)\).
		\[(x e^x) y' + (x e^x) y \left[\frac{1}{x}+1\right] = (x e^x) e^x\]

		Integrate both sides with respect to \(x\).
		\[(x e^x) y = \int (x e^{2x})dx\]

		Integrate the right hand side using integration by parts. Let \(u = x, v' = e^{2x}\ \Rightarrow\ u' = 1, v = \frac{e^{2x}}{2}\).
		\begin{gather*}
			(x e^x) y = \frac{xe^{2x}}{2} - \int 1 \frac{e^{2x}}{2}dx\\
			(x e^x) y = \frac{xe^{2x}}{2} - \frac{e^{2x}}{4} + c\\
			y = \frac{e^x}{2} - \frac{e^{x}}{4x} + \frac{c}{x e^x}
		\end{gather*}

	\item[\textbf{5.}]


	\item[\textbf{7.}]


	\item[\textbf{9.}]


\end{enumerate}